Weidenbach_Book/IsaSAT/IsaSAT_Inprocessing_LLVM.thy
@@ -213,10 +213,32 @@ sepref_def ahm_get_marked_code
   unfolding ahm_get_marked_def
   by sepref
 
-lemmas [sepref_fr_rules] =
-  ahm_create_code.refine[FCOMP ahm_create_create, where R11 = encoded_irred_indices]
-  ahm_is_marked_code.refine[FCOMP ahm_is_marked_is_marked2[where R = encoded_irred_indices]]
-  ahm_get_marked_code.refine[FCOMP ahm_get_marked_get_marked[where R = encoded_irred_indices]]
+sepref_def ahm_empty_code
+  is \<open>ahm_empty\<close>
+  :: \<open>(larray64_assn (sint_assn' TYPE(64)))\<^sup>d \<rightarrow>\<^sub>a larray64_assn (sint_assn' TYPE(64))\<close>
+  unfolding ahm_empty_def
+  apply (annot_sint_const \<open>TYPE(64)\<close>)
+  apply (annot_snat_const \<open>TYPE(64)\<close>)
+  by sepref
+
+sepref_register empty
+lemma ahm_empty_empty:
+   \<open>(ahm_empty, empty) \<in> (array_hash_map_rel R) \<rightarrow> \<langle>array_hash_map_rel R\<rangle>nres_rel\<close>
+  unfolding ahm_empty_def empty_def uncurry_def fref_param1
+  apply (intro ext frefI nres_relI)
+  subgoal for x y
+    apply (refine_vcg WHILET_rule[where I = \<open>\<lambda>(i, CS). (\<forall>j<i. CS!j = 0) \<and> length CS = length x\<close> and R = \<open>measure (\<lambda>(i,_). length x -i)\<close>])
+    subgoal by auto
+    subgoal by auto
+    subgoal by auto
+    subgoal by auto
+    subgoal by auto
+    subgoal by auto
+    subgoal by auto
+    subgoal by (auto simp: array_hash_map_rel_def)
+    done
+  done
+
 
 sepref_def length_watchlist_full_impl
   is \<open>RETURN o length\<close>
@@ -354,11 +376,12 @@ proof -
     done
 qed
 
-thm ahm_set_marked_set_marked
 lemmas [sepref_fr_rules] =
   ahm_create_code.refine[FCOMP ahm_create_create, where R11 = encoded_irred_indices]
+  ahm_empty_code.refine[FCOMP ahm_empty_empty, where R19 = encoded_irred_indices]
   ahm_is_marked_code.refine[FCOMP ahm_is_marked_is_marked2[where R = encoded_irred_indices]]
   ahm_get_marked_code.refine[FCOMP ahm_get_marked_get_marked[where R = encoded_irred_indices]]
+  ahm_empty_code.refine[FCOMP ahm_empty_empty, where R19 = encoded_irred_indices]
   ahm_set_marked_code.refine[FCOMP ahm_set_marked_set_marked]
 
 definition length_watchlist_raw where
@@ -390,8 +413,6 @@ lemmas [unfolded inline_direct_return_node_case, llvm_code] =
 
 sepref_register create encoded_irred_index_set encoded_irred_index_get
 sepref_register uminus_lit:  "uminus :: nat literal \<Rightarrow> _"
-find_theorems isa_clause_remove_duplicate_clause_wl
-thm isa_clause_remove_duplicate_clause_wl_def
 
 lemma isa_clause_remove_duplicate_clause_wl_alt_def:
   \<open>isa_clause_remove_duplicate_clause_wl C S = (do{
@@ -460,15 +481,14 @@ sepref_def isa_binary_clause_subres_wl_impl
   by sepref
 
 sepref_def isa_deduplicate_binary_clauses_wl_code
-  is \<open>uncurry isa_deduplicate_binary_clauses_wl\<close>
-  :: \<open>[\<lambda>(L, S). length (get_clauses_wl_heur S) \<le> sint64_max \<and> learned_clss_count S \<le> uint64_max]\<^sub>a
-  unat_lit_assn\<^sup>k *\<^sub>a isasat_bounded_assn\<^sup>d \<rightarrow> isasat_bounded_assn\<close>
+  is \<open>uncurry2 isa_deduplicate_binary_clauses_wl\<close>
+  :: \<open>[\<lambda>((L, CS), S). length (get_clauses_wl_heur S) \<le> sint64_max \<and> learned_clss_count S \<le> uint64_max]\<^sub>a
+  unat_lit_assn\<^sup>k *\<^sub>a (hr_comp (larray_assn' TYPE(64) (sint_assn' TYPE(64))) (array_hash_map_rel encoded_irred_indices))\<^sup>d *\<^sub>a isasat_bounded_assn\<^sup>d \<rightarrow>
+  hr_comp (larray_assn' TYPE(64) (sint_assn' TYPE(64))) (array_hash_map_rel encoded_irred_indices) \<times>\<^sub>a isasat_bounded_assn\<close>
   supply [[goals_limit=1]]
   unfolding isa_deduplicate_binary_clauses_wl_def
     mop_polarity_st_heur_def[symmetric]
     mop_arena_status_st_def[symmetric]
-    length_watchlist_def[unfolded length_ll_def, symmetric]
-    length_watchlist_raw_def[symmetric]
     tri_bool_eq_def[symmetric]
     encoded_irred_index_set_def[symmetric]
     encoded_irred_index_irred_def[symmetric]
@@ -479,12 +499,51 @@ sepref_def isa_deduplicate_binary_clauses_wl_code
 sepref_register get_vmtf_heur_array_nth get_vmtf_heur_fst
   isa_deduplicate_binary_clauses_wl
 
+lemma Massign_split: \<open>do{ x \<leftarrow> (M :: _ nres); f x} = do{(a,b) \<leftarrow> M; f (a,b)}\<close>
+  by auto
+
+
+lemma isa_mark_duplicated_binary_clauses_as_garbage_wl2_alt_def:
+  \<open>isa_mark_duplicated_binary_clauses_as_garbage_wl2 S\<^sub>0 = (do {
+     let ns = get_vmtf_heur_array S\<^sub>0;
+    ASSERT (mark_duplicated_binary_clauses_as_garbage_pre_wl_heur S\<^sub>0);
+    CS \<leftarrow> create (length (get_watched_wl_heur S\<^sub>0));
+    (_, CS, S) \<leftarrow> WHILE\<^sub>T\<^bsup> \<lambda>(n,CS, S). get_vmtf_heur_array S\<^sub>0 = (get_vmtf_heur_array S)\<^esup>(\<lambda>(n, CS, S). n \<noteq> None \<and> get_conflict_wl_is_None_heur S)
+      (\<lambda>(n, CS, S). do {
+        ASSERT (n \<noteq> None);
+        let A = the n;
+        ASSERT (A < length (get_vmtf_heur_array S));
+        ASSERT (A \<le> uint32_max div 2);
+        let skip = False;
+        if skip then RETURN (get_next (get_vmtf_heur_array S ! A), CS, S)
+        else do {
+          ASSERT (length (get_clauses_wl_heur S) \<le> length (get_clauses_wl_heur S\<^sub>0) \<and> learned_clss_count S \<le> learned_clss_count S\<^sub>0);
+          (CS, S) \<leftarrow> isa_deduplicate_binary_clauses_wl (Pos A) CS S;
+          ASSERT (length (get_clauses_wl_heur S) \<le> length (get_clauses_wl_heur S\<^sub>0) \<and> learned_clss_count S \<le> learned_clss_count S\<^sub>0);
+          (CS, S) \<leftarrow> isa_deduplicate_binary_clauses_wl (Neg A) CS S;
+          ASSERT (ns = get_vmtf_heur_array S);
+         RETURN (get_next (get_vmtf_heur_array S ! A), CS, S)
+       }
+     })
+     (Some (get_vmtf_heur_fst S\<^sub>0), CS, S\<^sub>0);
+    RETURN S
+          })\<close>
+   unfolding isa_mark_duplicated_binary_clauses_as_garbage_wl2_def
+   apply (simp add: case_prod_beta)
+   apply (subst Massign_split[of \<open>_ :: (_ \<times> isasat) nres\<close>])
+   apply (subst (2) Massign_split[of \<open>_ :: (_ \<times> isasat) nres\<close>])
+   unfolding prod.simps
+   apply simp
+   done
+
 sepref_def isa_deduplicate_binary_clauses_code
   is isa_mark_duplicated_binary_clauses_as_garbage_wl2
   :: \<open>[\<lambda>S. length (get_clauses_wl_heur S) \<le> sint64_max \<and> learned_clss_count S \<le> uint64_max]\<^sub>a
      isasat_bounded_assn\<^sup>d \<rightarrow> isasat_bounded_assn\<close>
-  unfolding isa_mark_duplicated_binary_clauses_as_garbage_wl2_def
+  unfolding isa_mark_duplicated_binary_clauses_as_garbage_wl2_alt_def
     get_vmtf_heur_array_nth_def[symmetric] atom.fold_option nres_monad3
+    length_watchlist_def[unfolded length_ll_def, symmetric]
+    length_watchlist_raw_def[symmetric]
   apply (rewrite at \<open>let _ = get_vmtf_heur_array _ in _\<close> Let_def)
   apply (rewrite at \<open>let _ = False in _\<close> Let_def)
   unfolding if_False nres_monad3
